format-version: 1.2
data-version: ddpheno/releases/2020-06-19/imports/ddanat_import.owl
ontology: ddpheno/imports/ddanat_import

[Term]
id: DDANAT:0000002
name: vegetative amoebae
namespace: Dictyostelium_discoideum_anatomy
def: "Unicellular haploid myxamoebae that feeds on bacteria by phagocytosis and divides by binary fission. The size of vegetative cells range from 12-20 microns by 8-12 microns. The cells exhibit a roughly rounded but rather irregular shape." [DDB:pg, PMID:4338436]
synonym: "amoebae" BROAD []
synonym: "vegetative cell" EXACT []
is_a: DDANAT:0000083 ! Dictyostelium discoideum single cell organism
relationship: develops_from DDANAT:0000414 ! spore
relationship: part_of DDANAT:0000013 ! stream

[Term]
id: DDANAT:0000003
name: aggregation territory
namespace: Dictyostelium_discoideum_anatomy
def: "Area covered by a group of chemotactic cells converging toward the same aggregation center. Can reach a diameter of up to 1 cm." [DDB:pg, PMID:14458213, PMID:20268085]
is_a: DDANAT:0010082 ! whole organism

[Term]
id: DDANAT:0000004
name: loose aggregate
namespace: Dictyostelium_discoideum_anatomy
def: "First adherent mass of cells observed during development, relatively flat with indistinct borders." [DDB:pg]
synonym: "loose mound" EXACT []
is_a: DDANAT:0010082 ! whole organism
relationship: develops_from DDANAT:0000003 ! aggregation territory

[Term]
id: DDANAT:0000005
name: mound
namespace: Dictyostelium_discoideum_anatomy
def: "Hemispherical structure composed of post-aggregative cells that are undergoing differentiation." [DDB:pg, PMID:20268085]
synonym: "pseudoplasmodium" BROAD [PMID:18366659]
synonym: "tight aggregate" EXACT []
synonym: "tight mound" EXACT []
is_a: DDANAT:0010082 ! whole organism
relationship: develops_from DDANAT:0000004 ! loose aggregate

[Term]
id: DDANAT:0000006
name: tipped mound
namespace: Dictyostelium_discoideum_anatomy
def: "Hemispherical structure composed of post-aggregative cells that are undergoing differentiation and that have formed a tip." [DDB:pg, PMID:20268085]
synonym: "pseudoplasmodium" BROAD []
synonym: "tipped aggregate" EXACT [PMID:7553878]
is_a: DDANAT:0010082 ! whole organism
relationship: develops_from DDANAT:0000005 ! mound

[Term]
id: DDANAT:0000007
name: standing slug
namespace: Dictyostelium_discoideum_anatomy
def: "Cylindrical structure that is formed by elongation of the mound under the control of the tip. The elongating tip is called the first finger." [DDB:pg, PMID:18366659]
comment: Synonym from Kessin book p. 166.
synonym: "finger" EXACT []
synonym: "first finger" NARROW []
synonym: "pseudoplasmodium" BROAD []
xref: ISBN:0521583640
is_a: DDANAT:0010082 ! whole organism
relationship: develops_from DDANAT:0000006 ! tipped mound

[Term]
id: DDANAT:0000008
name: migratory slug
namespace: Dictyostelium_discoideum_anatomy
def: "When the conditions are not optimal for the completion of development, the standing slug bends from a vertical position to a horizontal position, producing a migratory that slug has the ability to migrate towards more favorable environmental conditions. The slug is cylindrical in shape with a rounded, tapering region at its anterior end that is raised with respect to the substratum. It usually measures between 0.8 to 1.2 mm in length with a diameter of 0.15 to 0.25 mm. Slugs sense and respond to light, temperature and acidity, and do not enter culmination until the conditions are optimal. The slug can move at a speed of 0.5 to 2 mm per hour. A trail of slime is deposited on the surface during migration." [DDB:pg, PMID:2513127, PMID:8223266]
synonym: "pseudoplasmodium" BROAD [PMID:18366659]
is_a: DDANAT:0010082 ! whole organism
relationship: develops_from DDANAT:0000007 ! standing slug

[Term]
id: DDANAT:0000009
name: early culminant
namespace: Dictyostelium_discoideum_anatomy
def: "Structure formed after the arrest of slug migration formed when cells of the posterior region of the slug move under the tip. Stalk tube formation is initiated at this stage." [DDB:pg, PMID:18366659, PMID:1879341]
synonym: "culminant" BROAD []
synonym: "mexican hat" NARROW []
synonym: "pseudoplasmodium" BROAD [PMID:18366659]
is_a: DDANAT:0010082 ! whole organism
relationship: develops_from DDANAT:0000007 ! standing slug

[Term]
id: DDANAT:0000010
name: mid culminant
namespace: Dictyostelium_discoideum_anatomy
def: "Structure in which stalk tube formation has progressed down the prespore zone. Basal disc formation begins at this stage, with the migration of pstA and pstB cells to the lower part of the culminant to form the basal disc." [DDB:pg, PMID:9799430]
synonym: "culminant" BROAD []
synonym: "pseudoplasmodium" BROAD [PMID:18366659]
is_a: DDANAT:0010082 ! whole organism
relationship: develops_from DDANAT:0000009 ! early culminant

[Term]
id: DDANAT:0000011
name: late culminant
namespace: Dictyostelium_discoideum_anatomy
def: "Structure in which stalk tube formation has progressed down to the basal disc. The sorogen ascents up the stalk to it apical position during this stage. Terminal differentiation occurs at this stage: death of the stalk cells and encapsulation of the spores." [DDB:pg, PMID:1879341]
comment: Kessin book p. 201.
synonym: "culminant" BROAD []
synonym: "pseudoplasmodium" RELATED [PMID:18366659]
xref: ISBN:0521583640
is_a: DDANAT:0010082 ! whole organism
relationship: develops_from DDANAT:0000010 ! mid culminant

[Term]
id: DDANAT:0000012
name: fruiting body
namespace: Dictyostelium_discoideum_anatomy
def: "Dicty asexual organism which is terminally differentiated and consists of a long stalk on top of which sits the sorus that contains spores. The mature fruiting body measures between 1.5 to 3 mm in height." [DDB:18366659, DDB:pg]
comment: Synonym from Kessin book p. 12-13.
synonym: "sorocarp" EXACT []
xref: ISBN:0521583640
is_a: DDANAT:0010082 ! whole organism
relationship: develops_from DDANAT:0000011 ! late culminant

[Term]
id: DDANAT:0000013
name: stream
namespace: Dictyostelium_discoideum_anatomy
def: "Macroscopic appearance of groups of chemotactic cells orienting themselves in a head to tail fashion as they are migrating in the direction of the chemotactic stimulus to form aggregates." [DDB:18366659, DDB:pg]
synonym: "pseudoplasmodial stream" EXACT []
is_a: DDANAT:0010085 ! subdivision
relationship: part_of DDANAT:0000003 ! aggregation territory

[Term]
id: DDANAT:0000017
name: prespore region of the tipped mound
namespace: Dictyostelium_discoideum_anatomy
def: "Region of the tipped mound mostly composed of prespore cells. In addition to prespore cells, the prespore region contains anterior-like cells (ALC) that express ecmA and/or ecmB." [DDB:pg]
synonym: "psp region of the tipped mound" EXACT []
is_a: DDANAT:0000086 ! prespore region
relationship: develops_from DDANAT:0000005 ! mound
relationship: part_of DDANAT:0000006 ! tipped mound

[Term]
id: DDANAT:0000024
name: prespore region of the standing slug
namespace: Dictyostelium_discoideum_anatomy
def: "Region of the standing slug mostly composed of prespore cells. In addition to prespore cells, the prespore region contains anterior-like cells (ALC) that express ecmA and/or ecmB. The prespore region occupies about three quarters of the organism." [DDB:pg]
synonym: "psp region of the standing slug" EXACT []
is_a: DDANAT:0000086 ! prespore region
relationship: develops_from DDANAT:0000017 ! prespore region of the tipped mound
relationship: part_of DDANAT:0000007 ! standing slug

[Term]
id: DDANAT:0000033
name: prespore region of the migratory slug
namespace: Dictyostelium_discoideum_anatomy
def: "Region of the migratory slug composed mostly of prespore cells. In addition to prespore cells, the prespore region contains anterior-like cells (ALC) that express ecmA and/or ecmB. The prespore region occupies about three quarters of the organism." [DDB:pg]
synonym: "psp region of the migratory slug" BROAD []
is_a: DDANAT:0000086 ! prespore region
relationship: develops_from DDANAT:0000024 ! prespore region of the standing slug
relationship: part_of DDANAT:0000008 ! migratory slug

[Term]
id: DDANAT:0000041
name: prespore region of the early culminant
namespace: Dictyostelium_discoideum_anatomy
def: "Region of the early culminant mostly composed of prespore cells. In addition to prespore cells, the prespore region contains anterior-like cells (ALC) that express ecmA and/or ecmB. The prespore region occupies about three quarters of the organism." [DDB:pg]
synonym: "psp region of the early culminant" EXACT []
is_a: DDANAT:0000086 ! prespore region
relationship: develops_from DDANAT:0000024 ! prespore region of the standing slug
relationship: part_of DDANAT:0000009 ! early culminant

[Term]
id: DDANAT:0000054
name: prespore region of the mid culminant
namespace: Dictyostelium_discoideum_anatomy
def: "Region of the mid culminant mostly composed of prespore cells. In addition to prespore cells, the prespore region contains anterior-like cells (ALC) that express ecmA and/or ecmB. The prespore region occupies about three quarters of the organism." [DDB:pg]
synonym: "psp region of the mid culminant" BROAD []
is_a: DDANAT:0000086 ! prespore region
relationship: develops_from DDANAT:0000041 ! prespore region of the early culminant
relationship: part_of DDANAT:0000010 ! mid culminant

[Term]
id: DDANAT:0000061
name: sorus of the late culminant
namespace: Dictyostelium_discoideum_anatomy
def: "Ovoid structure of the late culminant supported by the stalk and that contains the spores." [DDB:pg, ISBN:0198529171]
synonym: "spore head of the late culminant" EXACT []
is_a: DDANAT:0000094 ! sorus
relationship: develops_from DDANAT:0000054 ! prespore region of the mid culminant
relationship: part_of DDANAT:0000011 ! late culminant

[Term]
id: DDANAT:0000070
name: sorus of the fruiting body
namespace: Dictyostelium_discoideum_anatomy
def: "Structure of the fruiting body supported by the stalk and that contains the spores. The sorus is 125-300 microns in diameter, lemon-shaped, and grayish white to pale yellow in color." [DDB:pg]
synonym: "spore head of the fruiting body" EXACT []
is_a: DDANAT:0000094 ! sorus
relationship: develops_from DDANAT:0000061 ! sorus of the late culminant
relationship: part_of DDANAT:0000012 ! fruiting body

[Term]
id: DDANAT:0000083
name: Dictyostelium discoideum single cell organism
namespace: Dictyostelium_discoideum_anatomy
def: "Cell that is an individual member of the species Dictyostelium discoideum." [CARO:MAH, DDB:PG]
synonym: "D. discoideum single cell organism" EXACT []
xref: CARO:0000064
is_a: DDANAT:0000401 ! cell

[Term]
id: DDANAT:0000086
name: prespore region
namespace: Dictyostelium_discoideum_anatomy
def: "Region mostly composed of prespore cells. In addition to prespore cells, the prespore region contains anterior-like cells (ALC) that express ecmA and/or ecmB. The prespore region occupies about three quarters of the organism." [DDB:pg]
synonym: "psp region" EXACT []
is_a: DDANAT:0010085 ! subdivision

[Term]
id: DDANAT:0000094
name: sorus
namespace: Dictyostelium_discoideum_anatomy
def: "Ovoid structure supported by the stalk and that contains the spores." [DDB:pg]
synonym: "spore head" EXACT []
is_a: DDANAT:0010085 ! subdivision

[Term]
id: DDANAT:0000401
name: cell
namespace: Dictyostelium_discoideum_anatomy
def: "Anatomical structure that has as its parts a maximally connected cell compartment surrounded by a plasma membrane." [CARO:MAH]
is_a: DDANAT:0010001 ! Dictyostelium discoideum anatomical structure

[Term]
id: DDANAT:0000402
name: chemotactic amoeboid cell
namespace: Dictyostelium_discoideum_anatomy
def: "Starved cell that secretes and responds to chemoattractants (cAMP)." [DDB:pg, PMID:4338436]
synonym: "amoebae" BROAD []
is_a: DDANAT:0000083 ! Dictyostelium discoideum single cell organism
relationship: develops_from DDANAT:0000414 ! spore
relationship: part_of DDANAT:0000013 ! stream

[Term]
id: DDANAT:0000403
name: aggregate cell
namespace: Dictyostelium_discoideum_anatomy
def: "Differentiating cell composing the aggregate that has acquired adhesive properties." [DDB:pg]
is_a: DDANAT:0000401 ! cell
relationship: develops_from DDANAT:0000402 ! chemotactic amoeboid cell
relationship: part_of DDANAT:0000003 ! aggregation territory
relationship: part_of DDANAT:0000004 ! loose aggregate
relationship: part_of DDANAT:0000005 ! mound

[Term]
id: DDANAT:0000405
name: prespore cell
namespace: Dictyostelium_discoideum_anatomy
def: "Cell that is undergoing differentiation to become a spore. Characterized by the presence of prespore vesicles (PV)." [DDB:pg, PMID:4330277]
synonym: "psp cell" EXACT []
is_a: DDANAT:0000401 ! cell
relationship: develops_from DDANAT:0000403 ! aggregate cell
relationship: part_of DDANAT:0000004 ! loose aggregate
relationship: part_of DDANAT:0000017 ! prespore region of the tipped mound
relationship: part_of DDANAT:0000024 ! prespore region of the standing slug
relationship: part_of DDANAT:0000033 ! prespore region of the migratory slug
relationship: part_of DDANAT:0000041 ! prespore region of the early culminant
relationship: part_of DDANAT:0000054 ! prespore region of the mid culminant
relationship: part_of DDANAT:0000061 ! sorus of the late culminant

[Term]
id: DDANAT:0000414
name: spore
namespace: Dictyostelium_discoideum_anatomy
def: "Dormant cell protected by a tri-layer spore coat. The spore has an elliptical shape and is approximately 6-9 microns by 3 microns." [DDB:pg, PMID:4338436]
synonym: "spore cell" EXACT []
is_a: DDANAT:0000083 ! Dictyostelium discoideum single cell organism
relationship: develops_from DDANAT:0000405 ! prespore cell
relationship: part_of DDANAT:0000070 ! sorus of the fruiting body

[Term]
id: DDANAT:0010001
name: Dictyostelium discoideum anatomical structure
namespace: Dictyostelium_discoideum_anatomy
alt_id: DDANAT:0000001
def: "Material anatomical entity that has inherent 3D shape and is generated by coordinated expression of the Dictyostelium discoideum genome." [CARO:MAH]

[Term]
id: DDANAT:0010082
name: whole organism
namespace: Dictyostelium_discoideum_anatomy
alt_id: DDANAT:0000082
def: "Anatomical structure that is an individual member of the Dictyostelium discoideum species and consists of more than one cell." [CARO:MAH]
xref: CARO:0000012
is_a: DDANAT:0010001 ! Dictyostelium discoideum anatomical structure

[Term]
id: DDANAT:0010085
name: subdivision
namespace: Dictyostelium_discoideum_anatomy
alt_id: DDANAT:0000085
def: "Anatomical structure which is a primary subdivision of whole Dictyostelium organism. The mereological sum of these is the whole organism." [DDB:pg]
xref: CARO:0000032
is_a: DDANAT:0010001 ! Dictyostelium discoideum anatomical structure

[Typedef]
id: develops_from
name: develops_from
namespace: Dictyostelium_discoideum_anatomy

[Typedef]
id: part_of
name: part of
namespace: Dictyostelium_discoideum_anatomy
is_transitive: true

